theories/logrel/F_mu_ref_conc/examples/fact.v
@@ -1,0 +1,250 @@
+From iris.proofmode Require Import tactics.
+From iris_examples.logrel.F_mu_ref_conc Require Import
+     soundness_binary rules rules_binary.
+From iris.program_logic Require Import adequacy.
+
+Fixpoint mathfact n :=
+  match n with
+  | O => 1
+  | S m => n * (mathfact m)
+  end.
+
+Definition fact : expr :=
+  Rec (If (BinOp Eq (Var 1) (#n 0))
+          (#n 1)
+          (BinOp Mult (Var 1) (App (Var 0) (BinOp Sub (Var 1) (#n 1))))).
+
+Lemma fact_typed : [] ⊢ₜ fact : TArrow TNat TNat.
+Proof. repeat econstructor. Qed.
+
+Definition fact_acc_body : expr :=
+  Rec (Lam
+         (If (BinOp Eq (Var 2) (#n 0))
+             (Var 0)
+             (LetIn
+                (BinOp Mult (Var 2) (Var 0))
+                (LetIn
+                   (BinOp Sub (Var 3) (#n 1))
+                   (App (App (Var 3) (Var 0)) (Var 1))
+                )
+             )
+         )
+      ).
+
+Lemma fact_acc_body_typed : [] ⊢ₜ fact_acc_body : TArrow TNat (TArrow TNat TNat).
+Proof. repeat econstructor. Qed.
+
+Lemma fact_acc_body_subst f : fact_acc_body.[f] = fact_acc_body.
+Proof. by asimpl. Qed.
+
+Hint Rewrite fact_acc_body_subst : autosubst.
+
+Lemma fact_acc_body_unfold :
+  fact_acc_body =
+  Rec (Lam
+         (If (BinOp Eq (Var 2) (#n 0))
+             (Var 0)
+             (LetIn
+                (BinOp Mult (Var 2) (Var 0))
+                (LetIn
+                   (BinOp Sub (Var 3) (#n 1))
+                   (App (App (Var 3) (Var 0)) (Var 1))
+                )
+             )
+         )
+      ).
+Proof. trivial. Qed.
+
+Global Typeclasses Opaque fact_acc_body.
+Global Opaque fact_acc_body.
+
+Definition fact_acc : expr :=
+  Lam (App (App fact_acc_body (Var 0)) (#n 1)).
+
+Lemma fact_acc_typed : [] ⊢ₜ fact_acc : TArrow TNat TNat.
+Proof.
+  repeat econstructor.
+  apply (closed_context_weakening [_] []); eauto.
+  apply fact_acc_body_typed.
+Qed.
+
+Section fact_equiv.
+  Context `{heapIG Σ, cfgSG Σ}.
+
+  Lemma fact_fact_acc_refinement :
+    [] ⊨ fact ≤log≤ fact_acc : (TArrow TNat TNat).
+  Proof.
+    iIntros (? vs ρ _) "[#HE HΔ]".
+    iDestruct (interp_env_length with "HΔ") as %?; destruct vs; simplify_eq.
+    rewrite !empty_env_subst.
+    iClear "HΔ". simpl.
+    iIntros (j K) "Hj"; simpl.
+    iApply wp_value; iExists (LamV _); iFrame.
+    rewrite /= -/fact.
+    iAlways. iIntros ([? ?] [n [? ?]]); simpl in *; simplify_eq; simpl.
+    clear j K.
+    iIntros (j K) "Hj"; simpl.
+    iMod (do_step_pure with "[$Hj]") as "Hj"; auto.
+    asimpl.
+    iApply (wp_mono _ _ _ (λ v, j ⤇ fill K (#n (mathfact n)) ∗ ⌜v = #nv (mathfact n)⌝))%I.
+    { iIntros (?) "[? %]"; iExists (#nv _); iFrame; eauto. }
+    replace (fill K (#n mathfact n)) with (fill K (#n (1 * mathfact n)))
+      by by repeat f_equal; lia.
+    generalize 1 as l => l.
+    iInduction n as [|n] "IH" forall (l).
+    - iApply wp_pure_step_later; auto.
+      iNext; simpl; asimpl.
+      rewrite fact_acc_body_unfold.
+      iMod (do_step_pure _ _ _ (AppLCtx _ :: _) with "[$Hj]") as "Hj"; auto.
+      rewrite -fact_acc_body_unfold.
+      simpl; asimpl.
+      iMod (do_step_pure with "[$Hj]") as "Hj"; auto.
+      iApply (wp_bind (fill [IfCtx _ _])).
+      iApply wp_pure_step_later; auto.
+      iNext; simpl.
+      iApply wp_value. simpl.
+      iMod (do_step_pure _ _ _ (IfCtx _ _ :: _) with "[$Hj]") as "Hj"; auto.
+      simpl.
+      iApply wp_pure_step_later; auto.
+      iNext; simpl.
+      iMod (do_step_pure with "[$Hj]") as "Hj"; auto.
+      iApply wp_value.
+      replace (l * 1) with l by lia.
+      auto.
+    - iApply wp_pure_step_later; auto.
+      iNext; simpl; asimpl.
+      rewrite fact_acc_body_unfold.
+      iMod (do_step_pure _ _ _ (AppLCtx _ :: _) with "[$Hj]") as "Hj"; auto.
+      rewrite -fact_acc_body_unfold.
+      simpl; asimpl.
+      iMod (do_step_pure with "[$Hj]") as "Hj"; auto.
+      iApply (wp_bind (fill [IfCtx _ _])).
+      iApply wp_pure_step_later; auto.
+      iNext; simpl.
+      iApply wp_value. simpl.
+      iMod (do_step_pure _ _ _ (IfCtx _ _ :: _) with "[$Hj]") as "Hj"; auto.
+      simpl.
+      iApply wp_pure_step_later; auto.
+      iNext; simpl.
+      iMod (do_step_pure with "[$Hj]") as "Hj"; auto.
+      asimpl.
+      iApply (wp_bind (fill [BinOpRCtx _ (#nv _)])).
+      iApply (wp_bind (fill [AppRCtx (RecV _)])).
+      iApply wp_pure_step_later; auto.
+      iNext; simpl; iApply wp_value; simpl.
+      iMod (do_step_pure _ _ _ (LetInCtx _ :: _) with "[$Hj]") as "Hj"; auto.
+      simpl.
+      iMod (do_step_pure with "[$Hj]") as "Hj"; auto.
+      asimpl.
+      iMod (do_step_pure _ _ _ (LetInCtx _ :: _) with "[$Hj]") as "Hj"; auto.
+      simpl.
+      iMod (do_step_pure with "[$Hj]") as "Hj"; auto.
+      asimpl.
+      replace (n -0) with n by lia.
+      iApply wp_wand_r; iSplitL; first iApply ("IH" with "[Hj]"); eauto.
+      iIntros (v) "[H %]"; simplify_eq.
+      iApply wp_pure_step_later; auto.
+      iNext; simpl; iApply wp_value.
+      replace (l * (mathfact n + n * mathfact n)) with ((l + n * l) * mathfact n)
+        by lia.
+      iFrame; auto.
+  Qed.
+
+  Lemma fact_acc_fact_refinement :
+    [] ⊨ fact_acc ≤log≤ fact : (TArrow TNat TNat).
+  Proof.
+    iIntros (? vs ρ _) "[#HE HΔ]".
+    iDestruct (interp_env_length with "HΔ") as %?; destruct vs; simplify_eq.
+    rewrite !empty_env_subst.
+    iClear "HΔ". simpl.
+    iIntros (j K) "Hj"; simpl.
+    iApply wp_value; iExists (RecV _); iFrame.
+    iAlways. iIntros ([? ?] [n [? ?]]); simpl in *; simplify_eq; simpl.
+    clear j K.
+    iIntros (j K) "Hj"; simpl.
+    iApply wp_pure_step_later; auto.
+    iNext; asimpl.
+    rewrite -/fact.
+    iApply (wp_mono _ _ _ (λ v, j ⤇ fill K (#n (mathfact n)) ∗ ⌜v = #nv (1 * mathfact n)⌝))%I.
+    { replace (1 * mathfact n) with (mathfact n) by lia.
+      iIntros (?) "[? %]"; iExists (#nv _); iFrame; eauto. }
+    generalize 1 as l => l.
+    iInduction n as [|n] "IH" forall (K l).
+    - rewrite fact_acc_body_unfold.
+      iApply (wp_bind (fill [AppLCtx _])).
+      iApply wp_pure_step_later; auto.
+      rewrite -fact_acc_body_unfold.
+      iNext; simpl; asimpl.
+      iApply wp_value; simpl.
+      iApply wp_pure_step_later; auto.
+      iNext; simpl; asimpl.
+      iMod (do_step_pure with "[$Hj]") as "Hj"; auto.
+      simpl; asimpl.
+      iMod (do_step_pure _ _ _ (IfCtx _ _ :: _) with "[$Hj]") as "Hj"; auto.
+      iApply (wp_bind (fill [IfCtx _ _])).
+      iApply wp_pure_step_later; auto.
+      iNext; simpl.
+      iApply wp_value. simpl.
+      iMod (do_step_pure with "[$Hj]") as "Hj"; auto.
+      iApply wp_pure_step_later; auto.
+      iNext; simpl.
+      iApply wp_value.
+      replace (l * 1) with l by lia; auto.
+    - rewrite {2}fact_acc_body_unfold.
+      iApply (wp_bind (fill [AppLCtx _])).
+      iApply wp_pure_step_later; auto.
+      rewrite -fact_acc_body_unfold.
+      iNext; simpl; asimpl.
+      iApply wp_value; simpl.
+      iApply wp_pure_step_later; auto.
+      iNext; simpl; asimpl.
+      iMod (do_step_pure with "[$Hj]") as "Hj"; auto.
+      simpl.
+      iApply (wp_bind (fill [IfCtx _ _])).
+      iApply wp_pure_step_later; auto.
+      iNext; simpl.
+      iApply wp_value. simpl.
+      iMod (do_step_pure _ _ _ (IfCtx _ _ :: _) with "[$Hj]") as "Hj"; auto.
+      simpl.
+      iApply wp_pure_step_later; auto.
+      iNext; simpl.
+      iMod (do_step_pure with "[$Hj]") as "Hj"; auto.
+      iMod (do_step_pure _ _ _ (AppRCtx (RecV _):: BinOpRCtx _ (#nv _) :: _)
+              with "[$Hj]") as "Hj"; eauto.
+      simpl.
+      iApply (wp_bind (fill [LetInCtx _])).
+      iApply wp_pure_step_later; auto.
+      iNext; simpl; iApply wp_value; simpl.
+      iApply wp_pure_step_later; auto.
+      iNext; simpl. asimpl.
+      iApply (wp_bind (fill [LetInCtx _])).
+      iApply wp_pure_step_later; auto.
+      iNext; simpl; iApply wp_value; simpl.
+      iApply wp_pure_step_later; auto.
+      iNext; simpl. asimpl.
+      replace (n -0) with n by lia.
+      iApply wp_fupd.
+      iApply wp_wand_r; iSplitL;
+        first iApply ("IH" $! (BinOpRCtx _ (#nv _) :: K) with "[$Hj]"); eauto.
+      iIntros (v) "[Hj %]"; simplify_eq.
+      simpl.
+      iMod (do_step_pure with "[$Hj]") as "Hj"; auto.
+      simpl.
+      iModIntro. iFrame.
+      eauto with lia.
+  Qed.
+
+End fact_equiv.
+
+Theorem fact_ctx_equiv :
+  [] ⊨ fact ≤ctx≤ fact_acc : (TArrow TNat TNat) ∧
+  [] ⊨ fact_acc ≤ctx≤ fact : (TArrow TNat TNat).
+Proof.
+  set (Σ := #[invΣ ; gen_heapΣ loc val ; GFunctor (auth.authR cfgUR)]).
+  set (HG := soundness_unary.HeapPreIG Σ _ _).
+  split.
+  - eapply (binary_soundness Σ _); auto using fact_acc_typed, fact_typed.
+    intros; apply fact_fact_acc_refinement.
+  -  eapply (binary_soundness Σ _); auto using fact_acc_typed, fact_typed.
+    intros; apply fact_acc_fact_refinement.
+Qed.
